
# Hello

$$
\begin{align}
2x^2 + 3(x-1)(x-2) & = 2x^2 + 3(x^2-3x+2)\\ \nonumber &= 2x^2 + 3x^2 - 9x + 6\\ &= 5x^2 - 9x + 6
\end{align}
$$

Here is a simple flow chart:

```mermaid
graph TD;
    A-->B;
    A-->C;
    B-->D;
    C-->D;
```

First Header  | Second Header
------------- | -------------
Content Cell  | Content Cell
Content Cell  | Content Cell


```mermaid
classDiagram
classA --|> classB : Inheritance
classC --* classD : Composition
classE --o classF : Aggregation
classG --> classH : Association
classI -- classJ : Link(Solid)
classK ..> classL : Dependency
classM ..|> classN : Realization
classO .. classP : Link(Dashed)
```
